seal u64_le / u32_le.
very few proofs actually need to open them, yet they were getting
opened by tactics like injection, even tho they were Opaque.
most proofs should just rely on lemmas about their length.
i've ported some proofs over, but still have more to go.

src/Helpers/Word/LittleEndian.v
@@ -1,4 +1,6 @@
+From Coq Require Import ssreflect.
 From stdpp Require Import prelude.
+From Perennial Require Import base.
 From coqutil Require Import Datatypes.HList.
 From coqutil.Word Require Import Interface Properties.
 From Perennial.Helpers.Word Require Import Integers Properties.
@@ -9,11 +11,23 @@ From Perennial Require Import Helpers.LittleEndian.
 Notation w64_bytes := 8%nat (only parsing).
 Notation w32_bytes := 4%nat (only parsing).
 
-(** 64-bit encoding *)
-Definition u64_le (x: u64) : list byte :=
+Definition u64_le_def (x: u64) : list byte :=
   let n := word.unsigned x in
   let t := split (byte:=w8_word_instance) w64_bytes n in
   tuple.to_list t.
+Program Definition u64_le := sealed @u64_le_def.
+Definition u64_le_unseal : u64_le = _ := seal_eq _.
+
+Definition u32_le_def (x: u32) : list byte :=
+  let n := word.unsigned x in
+  let t := split (byte:=w8_word_instance) w32_bytes n in
+  tuple.to_list t.
+Program Definition u32_le := sealed @u32_le_def.
+Definition u32_le_unseal : u32_le = _ := seal_eq _.
+
+Local Ltac unseal := rewrite ?u64_le_unseal ?u32_le_unseal.
+
+(** 64-bit encoding *)
 
 Definition le_to_u64 (l: list byte) : u64.
 Proof.
@@ -23,12 +37,10 @@ Proof.
 Defined.
 
 Lemma u64_le_0 : u64_le (W64 0) = replicate w64_bytes (W8 0).
-Proof. reflexivity. Qed.
+Proof. unseal. reflexivity. Qed.
 
 Theorem u64_le_length x : length (u64_le x) = w64_bytes.
-Proof.
-  reflexivity.
-Qed.
+Proof. unseal. reflexivity. Qed.
 
 Theorem tuple_of_to_list_u64 {A} (t: tuple A w64_bytes) :
   tuple.of_list (tuple.to_list t) = t.
@@ -43,8 +55,9 @@ Qed.
 Theorem u64_le_to_word : forall x,
     le_to_u64 (u64_le x) = x.
 Proof.
+  unseal.
   intros x; simpl.
-  unfold le_to_u64, u64_le.
+  unfold le_to_u64, u64_le_def.
   rewrite -> tuple_of_to_list_u64.
   rewrite combine_split.
   change (Z.of_nat w64_bytes * 8) with 64.
@@ -52,15 +65,10 @@ Proof.
   rewrite word.of_Z_unsigned.
   done.
 Qed.
+
 (* end 64-bit code *)
 
-(* this block is a copy-paste of the above with s/64/32/ *)
 (** 32-bit encoding *)
-Definition u32_le (x: u32) : list byte :=
-  let n := word.unsigned x in
-  let t := split (byte:=w8_word_instance) w32_bytes n in
-  tuple.to_list t.
-Global Arguments u32_le : simpl never.
 
 Definition le_to_u32 (l: list byte) : u32.
 Proof.
@@ -70,12 +78,10 @@ Proof.
 Defined.
 
 Lemma u32_le_0 : u32_le (W32 0) = replicate w32_bytes (W8 0).
-Proof. reflexivity. Qed.
+Proof. unseal. reflexivity. Qed.
 
 Theorem u32_le_length x : length (u32_le x) = w32_bytes.
-Proof.
-  reflexivity.
-Qed.
+Proof. unseal. reflexivity. Qed.
 
 Theorem tuple_of_to_list_u32 {A} (t: tuple A w32_bytes) :
   tuple.of_list (tuple.to_list t) = t.
@@ -90,8 +96,9 @@ Qed.
 Theorem u32_le_to_word : forall x,
     le_to_u32 (u32_le x) = x.
 Proof.
+  unseal.
   intros x; simpl.
-  unfold le_to_u32, u32_le.
+  unfold le_to_u32, u32_le_def.
   rewrite -> tuple_of_to_list_u32.
   rewrite combine_split.
   change (Z.of_nat w32_bytes * 8) with 32.
@@ -99,6 +106,7 @@ Proof.
   rewrite word.of_Z_unsigned.
   done.
 Qed.
+
 (* end 32-bit code *)
 
 Global Instance u64_le_inj : Inj (=) (=) u64_le.
@@ -116,9 +124,7 @@ Qed.
 Lemma combine_unfold n b (t: HList.tuple byte n) :
   combine (S n) {| PrimitivePair.pair._1 := b; PrimitivePair.pair._2 := t |} =
   Z.lor (uint.Z b) (combine n t ≪ 8).
-Proof.
-  reflexivity.
-Qed.
+Proof. reflexivity. Qed.
 
 Theorem Zmod_small_bits_high p z n :
   0 <= z < 2 ^ p ->
@@ -139,7 +145,7 @@ Proof.
     let T := type of t in change T with (HList.tuple byte n) in *.
     rewrite combine_unfold.
     rewrite BitOps.or_to_plus.
-    { pose proof (IHn t).
+    2: { pose proof (IHn t).
       pose proof (word.unsigned_range b).
       split.
       { unfold Z.shiftl; simpl. lia. }
@@ -152,31 +158,27 @@ Proof.
     unfold Z.eqf; intros.
     rewrite Z.land_spec.
     rewrite Z.bits_0.
+    (* TODO: error here. *)
     destruct (decide (n0 < 0)).
-    { rewrite Z.testbit_neg_r; [ | lia ].
-      rewrite andb_false_l; auto.
-    }
+    { rewrite Z.testbit_neg_r; lia. }
     destruct (decide (n0 < 8)).
-    + rewrite Z.shiftl_spec_low; [ | lia ].
-      rewrite andb_false_r; auto.
-    + rewrite (Zmod_small_bits_high 8); [ | lia | lia ].
-      rewrite andb_false_l; auto.
+    + rewrite Z.shiftl_spec_low; lia.
+    + rewrite (Zmod_small_bits_high 8); lia.
 Qed.
 
 Lemma le_to_u64_le bs :
   length bs = 8%nat ->
   u64_le (le_to_u64 bs) = bs.
 Proof.
+  unseal.
   intros.
   do 8 (destruct bs; [ simpl in H; lia | ]).
   destruct bs; [ clear H | simpl in H; lia ].
-  unfold u64_le, le_to_u64.
+  unfold u64_le_def, le_to_u64.
   rewrite word.unsigned_of_Z.
   rewrite wrap_small.
-  { rewrite LittleEndian.split_combine.
+  2: { rewrite LittleEndian.split_combine.
     simpl; auto. }
   cbv [length].
   apply combine_bound.
 Qed.
-
-Global Opaque u64_le.
